---
layout: "post"
title: "Binary heap"
category: datastructures

---


<script type="text/javascript" async
  src="https://cdn.mathjax.org/mathjax/latest/MathJax.js?config=TeX-MML-AM_CHTML">
</script>



[[toc]]
+ TOC
{:toc}  


# Heap

+ [Interesting Problem](http://www.geeksforgeeks.org/k-largestor-smallest-elements-in-an-array/)
+ [There exits multiple types of heaps. We are talking about Binary Heap](https://en.wikipedia.org/wiki/Heap_data_structure)
+ [Binary Heap Theory](https://www.cs.cmu.edu/~adamchik/15-121/lectures/Binary%20Heaps/heaps.html)


## Some Characteristics 
 

### **Heap Is in the form of a binary tree**

### **N-th level in heap has $$2^{n-1} elements$$**

### **N-th level in heap has one more element than all previous level elements summed up _Binary Number Characteristic_**  <-    $$2^{n}=\sum_{i=0}^{n-1}{2^{i}}+1$$ 

_Proof by induction_

+ This is correct when n=3 

+ Lets Perform the induction step with n+1


Left side: $$2^{n+1} = 2^{n} + 2^{n}$$

Right side $$=\sum_{i=0}^{n}{2^{i}}+1 =  2^{n} + \sum_{i=0}^{n-1}{2^{i}}+1$$

$$2^{n} + 2^{n} = 2^{n} + \sum_{i=0}^{n-1}{2^{i}}+1$$ <- Left Side = Right Side


### **N-th levels last element in heap is the $$2^{n}-1$$ -th element** 
### **j-th element in heap is in the floor(log(j)+1) level**.  $$2^{n}-1$$ -th element in heap is at n-th level
### **left child of j-th member is at 2 * j-th position ins heap, right is at 2*j+1 -th position**

**PROOF**
Last element in N-th level is $$2^{n}-1$$th element. In level N+1, it is $$2^{n+1}-1$$th element.
That means, when we go to from N-th level last element to

+ right child  $$2*2^{n}-1+1=2^{n+1}-1$$ <- Last element in N+1 level
+ left child $$2^{n}-1=2^{n+1}-2$$  <- Second to last element in N+1 level


First element in N-th level is $$2^{n-1}$$th element. In level N+1, it is $$2^{n}$$th element.

+ right $$2*2^{n-1}+1=2^{n}+1$$ <-Second to First element in n+1 level
+ left $$2*2^{n-1}=2^{n}$$ <- First element in n+1 level


If we go to second to last element in N-th level, it childs

+ right child  $$2*2^{n}-2 +1=2^{n+1}-3$$ <- 3. from last element in N+1 level
+ left child $$2^{n}-2=2^{n+1}-4$$  <- 4. from last to last element in N+1 level




